GreedyDeriv/Examples.lean
@@ -17,76 +17,97 @@ instance : Coe String (Loc Char) where
 
 -- a + ab
 def r : Regex (Char) := plus 'a' "ab"
-#eval r.matchEnd "ab" = r.gmatch "ab"
+#eval r.matchEnd "ab"
+#eval r.gmatch "ab"
 
 -- (a + ab)*
 def r2 : Regex (Char) := (plus 'a' "ab").star
-#eval r2.matchEnd "aab" = r2.gmatch "aab"
+#eval r2.matchEnd "aab"
+#eval r2.gmatch "aab"
 
 -- c + ab
 def r3 : Regex (Char) := plus 'c' (mul 'a' 'b')
-#eval r3.matchEnd "ab" = r3.gmatch "ab"
+#eval r3.matchEnd "ab"
+#eval r3.gmatch "ab"
 
 -- (a + aa)a
 def r4 : Regex (Char) := (plus 'a' "aa").mul 'a'
-#eval r4.matchEnd "aaa" = r4.gmatch "aaa"
+#eval r4.matchEnd "aaa"
+#eval r4.gmatch "aaa"
 
 -- a*a
 def r5 : Regex (Char) := (star 'a').mul 'a'
-#eval r5.matchEnd "aa" = r5.gmatch "aa"
+#eval r5.matchEnd "aa"
+#eval r5.gmatch "aa"
 
 -- (ε + b)*
 def r6 : Regex (Char) := (epsilon.plus 'b').star
-#eval r6.matchEnd "bb" = r6.gmatch "bb"
+#eval r6.matchEnd "bb"
+#eval r6.gmatch "bb"
 
 -- (ε + b)(ε + b)*
 def r6' : Regex (Char) := (epsilon.plus 'b').mul ((epsilon.plus 'b').star)
-#eval r6'.matchEnd "bb" = r6'.gmatch "bb"
+#eval r6'.matchEnd "bb"
+#eval r6'.gmatch "bb"
 
 -- (a + ε + b)*
 def r7 : Regex (Char) := (plus 'a' (epsilon.plus 'b')).star
-#eval r7.matchEnd "aaaabbb" = r7.gmatch "aaaabbb"
+#eval r7.matchEnd "aaaabbb"
+#eval r7.gmatch "aaaabbb"
 
 -- (ε + a)b
 def r8 : Regex (Char) := (epsilon.plus 'a').mul 'b'
-#eval r8.matchEnd "ab" = r8.gmatch "ab"
+#eval r8.matchEnd "ab"
+#eval r8.gmatch "ab"
 
 -- ((a + ε + b) + b)
 def r9 : Regex (Char) := Regex.plus ((plus 'a' epsilon).plus 'b') 'b'
-#eval r9.matchEnd "b" = r9.gmatch "b"
+#eval r9.matchEnd "b"
+#eval r9.gmatch "b"
 
 -- (ε + a)*b
 def r10 : Regex (Char) := ((Regex.plus epsilon 'a').star).mul 'b'
-#eval r10.matchEnd "ab" = r10.gmatch "ab"
+#eval r10.matchEnd "ab"
+#eval r10.gmatch "ab"
 
 -- (a + ε)*(ε + b)
 def r11 : Regex (Char) := ((Regex.plus 'a' epsilon).star).mul (Regex.plus (epsilon) 'b')
-#eval r11.matchEnd "ab" = r11.gmatch "ab"
+#eval r11.matchEnd "ab"
+#eval r11.gmatch "ab"
 
 -- (ε + a)*(ε + b)
 def r12 : Regex (Char) := ((Regex.plus epsilon 'a').star).mul (Regex.plus (epsilon) 'b')
-#eval r12.matchEnd "ab" = r12.gmatch "ab"
+#eval r12.matchEnd "ab"
+#eval r12.gmatch "ab"
 
 -- (ε + a)*ε
 def r12' : Regex (Char) := ((Regex.plus epsilon 'a').star).mul epsilon
-#eval r12'.gmatch "ab" = r12'.matchEnd "ab"
+#eval r12'.gmatch "ab"
+#eval r12'.matchEnd "ab"
 
 -- (a + ε + b)*b
 def r13 : Regex (Char) := ((Regex.plus 'a' (Regex.plus epsilon 'b')).star).mul 'b'
-#eval r13.matchEnd "bb" = r13.gmatch "bb"
+#eval r13.matchEnd "bb"
+#eval r13.gmatch "bb"
+#eval r13.prune
 
 -- (a + ε + b)*a
 def r13' : Regex (Char) := ((Regex.plus 'a' (Regex.plus epsilon 'b')).star).mul 'a'
-#eval r13'.matchEnd "aba" = r13'.gmatch "aba"
+#eval r13'.matchEnd "aba"
+#eval r13'.gmatch "aba"
 
 -- (aa + ε + a)*a
 def r13'' : Regex (Char) := ((Regex.plus "aa" (Regex.plus epsilon 'a')).star).mul 'a'
-#eval r13''.gmatch "aa" = r13''.matchEnd "aa"
+#eval r13''.gmatch "aa"
+#eval r13''.matchEnd "aa"
 
 -- (aa + aaa)*
 def r17 : Regex (Char) := (star (plus "aa" "aaa"))
-#eval r17.matchEnd "aaa" = r17.gmatch "aaa"
+#eval r17.matchEnd "aaa"
+#eval r17.gmatch "aaa"
 
--- (a + c* + b)*b
-def r19 : Regex Char := (mul (star (plus 'a' (plus (star 'c') 'b'))) 'b')
-#eval r19.gmatch "bb" = r19.matchEnd "bb"
+-- (a + c*** + b)*b
+def r19 : Regex Char := (mul (star (plus 'a' (plus (star 'c').star.star 'b'))) 'b')
+#eval r19.gmatch "bb"
+#eval r19.matchEnd "bb"
+#eval r19.prune
